module Transition.Concur.Cofinal.Lattice where

   open import ConcurrentSlicingCommon
   import Relation.Binary.EqReasoning as EqReasoning

   open import Action as ᴬ using (Action; Actionᵇ; Actionᶜ; inc); open ᴬ.Action
   open import Action.Concur using (_ᴬ⌣_; module _ᴬ⌣_; ᴬ⊖; ᴬγ); open _ᴬ⌣_
   open import Braiding.Proc.Lattice using (braid̂)
   open import Lattice using (Lattices); open Lattice.Prefixes ⦃...⦄
   open import Name as ᴺ using (Cxt; _+_)
   open import Proc as ᴾ using (Proc; Proc↱; Proc↲); open ᴾ.Proc
   open import Proc.Lattice as ᴾ̃ using (); open ᴾ̃.↓_; open ᴾ̃.↓⁻_
   import Proc.Ren
   open import Proc.Ren.Lattice renaming (_* to _*̃)
   open import Ren as ᴿ using (Ren); open ᴿ.Renameable ⦃...⦄
   open import Ren.Lattice using (_ᴿ+_; swap; push)
   open import Ren.Properties
   open import Transition as ᵀ using (_—[_-_]→_); open ᵀ._—[_-_]→_
   open import Transition.Concur using (Concur₁; module Concur₁; module Delta′; ⊖₁); open Concur₁
   open import Transition.Concur.Cofinal using (⋈̂[_,_,_]; γ₁)
   open import Transition.Lattice using (fwd; step)
   open import Transition.Ren using (_*ᵇ; _*ᶜ)
   open import Transition.Ren.Lattice using (ren-fwd-comm)

   braiding : ∀ {Γ} {a a′ : Action Γ} (𝑎 : a ᴬ⌣ a′) {Δ : Cxt} {P P′} → ⋈̂[ Γ , 𝑎 , Δ ] P P′ → ↓ P → ↓ P′
   braiding ˣ∇ˣ eq rewrite eq = idᶠ
   braiding ᵇ∇ᵇ {Δ} refl = (swap ᴿ+ Δ) *̃
   braiding ᵇ∇ᶜ refl = idᶠ
   braiding ᶜ∇ᵇ refl = idᶠ
   braiding ᶜ∇ᶜ refl = idᶠ
   braiding ᵛ∇ᵛ = braid̂

   open Delta′

   private
   -- Can't see a way to inline this into the proposition being proven.
      coerceCxt : ∀ {Γ} {a a′ : Action Γ} (𝑎 : a ᴬ⌣ a′) →
                  let Γ′ = Γ + inc a′ + inc (π₂ (ᴬ⊖ 𝑎)) in ∀ {P : Proc Γ′} → ↓ P → ↓ Proc↱ (sym (ᴬγ 𝑎)) P
      coerceCxt 𝑎 rewrite sym (ᴬγ 𝑎) = idᶠ

      reduce : ∀ {Γ} Δ (P P′ : Proc (Γ + 1 + Δ)) (a : Actionᵇ Γ) (a′ : Actionᶜ Γ) (γ : P ≡ P′) (P† : ↓ P) →
               braiding (ᵇ∇ᶜ {a = a} {a′}) {Δ} γ P† ≅ P†
      reduce = {!!}

   -- Not sure of the naming convention to use here.
   wibble : ∀ {Γ} {a a′ : Action Γ} {𝑎 : a ᴬ⌣ a′} {P R R′} {E : P —[ a - _ ]→ R} {E′ : P —[ a′ - _ ]→ R′}
            (𝐸 : E ⌣₁[ 𝑎 ] E′) → ∀ P′ →
            coerceCxt 𝑎 (π₂ (fwd (E/E′ (⊖₁ 𝐸)) (π₂ (fwd E′ P′)))) ≡
            braiding 𝑎 (γ₁ 𝐸) (π₂ (fwd (E′/E (⊖₁ 𝐸)) (π₂ (fwd E P′))))
   wibble _ ◻ = {!!}
   wibble {E = .E ᵇ│ ._} {E′ = ._ │ᵇ .F} (E ᵇ│ᵇ F) [ P │ Q ] = {!!}
   wibble (E ᵇ│ᶜ F) [ P │ Q ] = cong (λ Q′ → [ _ │ Q′ ]) (ren-fwd-comm F push Q)
   wibble (E ᶜ│ᵇ F) [ P │ Q ] = cong (λ P′ → [ P′ │ _ ]) (sym (ren-fwd-comm E push P))
   wibble (E ᶜ│ᶜ F) [ P │ Q ] = refl
   wibble (_│•ᵇ_ {y = y} {a = a} 𝐸 F) [ P │ Q ] with (ᴿ.pop y *ᵇ) (E/E′ (⊖₁ 𝐸))
   ... | pop-y*E/E′ rewrite pop∘push y a = {!!}
{-
   wibble (𝐸 │•ᶜ F) P₁ = {!!}
   wibble (E ᵇ│• 𝐸) P₁ = {!!}
   wibble (E ᶜ│• 𝐸) P₁ = {!!}
   wibble (𝐸 │ᵥᵇ F) P₁ = {!!}
   wibble (𝐸 │ᵥᶜ F) P₁ = {!!}
   wibble (E ᵇ│ᵥ 𝐸) P₁ = {!!}
   wibble (E ᶜ│ᵥ 𝐸) P₁ = {!!}
-}
   wibble (𝐸 ➕₁ Q) [ P ➕ _ ] = wibble 𝐸 P
   wibble {𝑎 = ˣ∇ˣ} (_ │ᵇᵇ 𝐸) [ P │ Q ] = {!!}
   wibble {𝑎 = ᵇ∇ᵇ} (_ │ᵇᵇ 𝐸) [ P │ Q ] = {!!}
   wibble {Γ} {a = a ᵇ} {a′ ᶜ} {E = P₀ │ᵇ F} {.P₀ │ᶜ F′} (._ │ᵇᶜ 𝐹) [ P │ Q ] =
      let nib : π₂ (fwd (E/E′ (⊖₁ 𝐹)) (π₂ (fwd F′ Q))) ≅ π₂ (fwd (E′/E (⊖₁ 𝐹)) (π₂ (fwd F Q)))
          nib = let open ≅-Reasoning in
             begin
                π₂ (fwd (E/E′ (⊖₁ 𝐹)) (π₂ (fwd F′ Q)))
             ≡⟨ wibble 𝐹 Q ⟩
                braiding (ᵇ∇ᶜ {a = a} {a′}) {0} (γ₁ 𝐹) (π₂ (fwd (E′/E (⊖₁ 𝐹)) (π₂ (fwd F Q))))
             ≅⟨ reduce 0 _ _ a a′ (γ₁ 𝐹) (π₂ (fwd (E′/E (⊖₁ 𝐹)) (π₂ (fwd F Q)))) ⟩
                π₂ (fwd (E′/E (⊖₁ 𝐹)) (π₂ (fwd F Q)))
             ∎
          jib : S′ (⊖₁ 𝐹) ≡ S (⊖₁ 𝐹)
          jib = let open ≅-Reasoning in ≅-to-≡ (
             begin
                S′ (⊖₁ 𝐹)
             ≅⟨ ≅-sym (Proc↲ refl (S′ (⊖₁ 𝐹))) ⟩
                Proc↱ refl (S′ (⊖₁ 𝐹))
             ≡⟨ sym (γ₁ 𝐹) ⟩
                S (⊖₁ 𝐹)
             ∎)
          spib : Proc (Γ + 1)
          spib = (ᴿ.push *) P₀ │ S′ (⊖₁ 𝐹)
          blah : ↓ spib
          blah = [ (push *̃) P │ π₂ (fwd (E/E′ (⊖₁ 𝐹)) (π₂ (fwd F′ Q))) ]
          zib : {Q′ : ↓ S′ (⊖₁ 𝐹)} {Q″ : ↓ S (⊖₁ 𝐹)} → Q′ ≅ Q″ → _≅_ {A = ↓ spib} [ (push *̃) P │ Q′ ] {{!!}} [ (push *̃) P │ Q″ ]
          zib = {!!}
          open ≅-Reasoning in ≅-to-≡ (
      begin
         [ (push *̃) P │ π₂ (fwd (E/E′ (⊖₁ 𝐹)) (π₂ (fwd F′ Q))) ]
      ≅⟨ {!!} ⟩ -- ≅-cong✴ ↓_ jib (λ Q′ → [ (push *̃) P │ Q′ ]) nib
         [ (push *̃) P │ π₂ (fwd (E′/E (⊖₁ 𝐹)) (π₂ (fwd F Q))) ]
      ≅⟨ ≅-sym (reduce 0 _ _ a a′ (cong₂ _│_ refl (γ₁ 𝐹))
         [ (push *̃) P │ π₂ (fwd (E′/E (⊖₁ 𝐹)) (π₂ (fwd F Q))) ]) ⟩
         braiding ᵇ∇ᶜ (cong₂ _│_ refl (γ₁ 𝐹)) [ (push *̃) P │ π₂ (fwd (E′/E (⊖₁ 𝐹)) (π₂ (fwd F Q))) ]
      ∎)
   wibble 𝐸 P = {!!}
{-
   wibble (P │ᶜᵇ 𝐸) P₁ = {!!}
   wibble (P │ᶜᶜ 𝐸) P₁ = {!!}
   wibble (P │ᵛᵛ 𝐸) P₁ = {!!}
   wibble (𝐸 ᵇᵇ│ Q) P₁ = {!!}
   wibble (𝐸 ᵇᶜ│ Q) P₁ = {!!}
   wibble (𝐸 ᶜᵇ│ Q) P₁ = {!!}
   wibble (𝐸 ᶜᶜ│ Q) P₁ = {!!}
   wibble (𝐸 ᵛᵛ│ Q) P₁ = {!!}
   wibble (𝐸 │• 𝐸₁) P₁ = {!!}
   wibble (𝐸 │•ᵥ 𝐸₁) P₁ = {!!}1
   wibble (𝐸 │ᵥ• 𝐸₁) P₁ = {!!}
   wibble (𝐸 │ᵥ 𝐸₁) P₁ = {!!}
   wibble (𝐸 │ᵥ′ 𝐸₁) P₁ = {!!}
   wibble (ν• 𝐸) P₁ = {!!}
   wibble (ν•ᵇ 𝐸) P₁ = {!!}
   wibble (ν•ᶜ 𝐸) P₁ = {!!}
   wibble (νᵇᵇ 𝐸) P₁ = {!!}
   wibble (νˣˣ 𝐸) P₁ = {!!}
   wibble (νᵇᶜ 𝐸) P₁ = {!!}
   wibble (νᶜᵇ 𝐸) P₁ = {!!}
   wibble (νᶜᶜ 𝐸) P₁ = {!!}
   wibble (νᵛᵛ 𝐸) P₁ = {!!}
   wibble (! 𝐸) P₁ = {!!}
-}
